src/riot/asn1/ASN1.Low.Value.BigInteger.fsti
@@ -1,0 +1,40 @@
+module ASN1.Low.Value.BigInteger
+
+open ASN1.Base
+open ASN1.Low.Base
+open ASN1.Low.Tag
+open ASN1.Low.Length
+open ASN1.Low.Value.OCTET_STRING
+open ASN1.Spec.Value.BigInteger
+module HS = FStar.HyperStack
+module HST = FStar.HyperStack.ST
+module MB = LowStar.Monotonic.Buffer
+module B = LowStar.Buffer
+module Cast = FStar.Int.Cast
+open LowParse.Low.Bytes
+
+open FStar.Integers
+module B32 = FStar.Bytes
+
+let serialize32_asn1_length_of_big_integer_backwards
+: serializer32_backwards (serialize_asn1_length_of_big_integer)
+= serialize32_asn1_length_of_bound_backwards 1ul (asn1_int32_max - 6ul)
+
+inline_for_extraction
+val serialize32_big_integer_as_octet_string_backwards
+  (len: asn1_value_int32_of_big_integer)
+: Tot (serializer32_backwards (serialize_big_integer_as_octet_string (v len)))
+
+noextract inline_for_extraction
+let parser_tag_of_big_integer_as_octet_string_impl
+  (x: big_integer_as_octet_string_t)
+: Tot (tg: (the_asn1_tag INTEGER & asn1_value_int32_of_big_integer)
+           { tg == parser_tag_of_big_integer_as_octet_string x })
+= let (.[]) = B32.index in
+  if ((dsnd x).[0] >= 0x80uy) then
+  ( (INTEGER, dfst x + 1ul) )
+  else
+  ( (INTEGER, dfst x) )
+
+val serialize32_big_integer_as_octet_string_TLV_backwards (_:unit)
+: Tot (serializer32_backwards (serialize_big_integer_as_octet_string_TLV))
