src/riot/asn1/ASN1.Low.Value.INTEGER.fsti
@@ -10,9 +10,23 @@ open FStar.Integers
 
 /// Implementation of length computation of `INTEGER` value's serialization
 inline_for_extraction
-val len_of_asn1_integer
+let len_of_asn1_integer
   (value: datatype_of_asn1_type INTEGER)
 : (len: asn1_value_int32_of_type INTEGER { v len == length_of_asn1_integer value } )
+= if      0l         <= value && value <= 0x7Fl      then
+  ( 1ul )
+  else if 0x7Fl       < value && value <= 0xFFl       then
+  ( 2ul )
+  else if 0xFFl       < value && value <= 0x7FFFl     then
+  ( 2ul )
+  else if 0x7FFFl     < value && value <= 0xFFFFl     then
+  ( 3ul )
+  else if 0xFFFFl     < value && value <= 0x7FFFFFl   then
+  ( 3ul )
+  else if 0x7FFFFFl   < value && value <= 0xFFFFFFl   then
+  ( 4ul )
+  else // if 0xFFFFFFl   < value && value <= 0x7FFFFFFFl then
+  ( 4ul )
 
 inline_for_extraction
 val serialize32_asn1_integer_backwards
