src/riot/asn1/ASN1.Spec.Value.CharacterString.fst
@@ -16,6 +16,8 @@ module B32 = FStar.Bytes
 
 #set-options "--z3rlimit 32 --fuel 0 --ifuel 0"
 
+(* ZT: I think we can leave this module exposed. *)
+
 noextract inline_for_extraction
 let len_of_character_string
   (t: character_string_type)
@@ -61,22 +63,34 @@ let string_prf
   | IA5_STRING -> ()
   | PRINTABLE_STRING -> ()
 
-let count_character t x
+noextract inline_for_extraction
+let count_character
+  (t: character_string_type)
+  (x: datatype_of_asn1_type t)
+: Tot (asn1_int32)
 = match t with
   | IA5_STRING -> count_ia5_character x
   | PRINTABLE_STRING -> count_printable_character x
 
-let parse_asn1_character_string t
+let parse_asn1_character_string
+  (t: character_string_type)
+: parser (parse_asn1_string_TLV_kind t) (datatype_of_asn1_type t)
 = match t with
   | IA5_STRING -> parse_asn1_ia5_string_TLV
   | PRINTABLE_STRING -> parse_asn1_printable_string_TLV
 
-let serialize_asn1_character_string t
+let serialize_asn1_character_string
+  (t: character_string_type)
+: serializer (parse_asn1_character_string t)
 = match t with
   | IA5_STRING -> serialize_asn1_ia5_string_TLV
   | PRINTABLE_STRING -> serialize_asn1_printable_string_TLV
 
-let parse_asn1_character_string_with_character_bound t lb ub
+let parse_asn1_character_string_with_character_bound
+  (t: character_string_type)
+  (lb: asn1_value_int32_of_type t)
+  (ub: asn1_value_int32_of_type t { lb <= ub })
+: parser (parse_asn1_string_TLV_kind t) (asn1_string_with_character_bound_t t (count_character t) lb ub)
 = match t with
   | IA5_STRING -> assert_norm (count_ia5_character == count_character IA5_STRING);
                   parse_asn1_ia5_string_TLV_with_character_bound lb ub
@@ -84,7 +98,11 @@ let parse_asn1_character_string_with_character_bound t lb ub
                -> assert_norm (count_printable_character == count_character PRINTABLE_STRING);
                   parse_asn1_printable_string_TLV_with_character_bound lb ub
 
-let serialize_asn1_character_string_with_character_bound t lb ub
+let serialize_asn1_character_string_with_character_bound
+  (t: character_string_type)
+  (lb: asn1_value_int32_of_type t)
+  (ub: asn1_value_int32_of_type t { lb <= ub })
+: serializer (parse_asn1_character_string_with_character_bound t lb ub)
 = match t with
   | IA5_STRING -> assert_norm (count_ia5_character == count_character IA5_STRING);
                   serialize_asn1_ia5_string_TLV_with_character_bound lb ub
@@ -92,7 +110,31 @@ let serialize_asn1_character_string_with_character_bound t lb ub
                -> assert_norm (count_printable_character == count_character PRINTABLE_STRING);
                   serialize_asn1_printable_string_TLV_with_character_bound lb ub
 
-let lemma_serialize_character_string_unfold t x
+let lemma_serialize_character_string_unfold
+  (t: character_string_type)
+  // (lb: asn1_value_int32_of_type t)
+  // (ub: asn1_value_int32_of_type t { lb <= ub })
+  // (x: asn1_string_with_character_bound_t t (count_character t) lb ub)
+  (x: datatype_of_asn1_type t)
+: Lemma (
+    match t with
+    | IA5_STRING -> predicate_serialize_asn1_string_TLV_unfold
+                     (IA5_STRING)
+                     (dfst)
+                     (filter_asn1_ia5_string)
+                     (synth_asn1_ia5_string)
+                     (synth_asn1_ia5_string_inverse)
+                     (lemma_synth_asn1_ia5_string_injective ())
+                     (x)
+    | PRINTABLE_STRING
+                 -> predicate_serialize_asn1_string_TLV_unfold
+                     (PRINTABLE_STRING)
+                     (dfst)
+                     (filter_asn1_printable_string)
+                     (synth_asn1_printable_string)
+                     (synth_asn1_printable_string_inverse)
+                     (lemma_synth_asn1_printable_string_injective ())
+                     (x))
 = match t with
   | IA5_STRING ->
                   // assert_norm ( t == IA5_STRING /\
@@ -109,7 +151,31 @@ let lemma_serialize_character_string_unfold t x
   | PRINTABLE_STRING
                -> lemma_serialize_asn1_printable_string_TLV_unfold x
 
-let lemma_serialize_character_string_size t x
+let lemma_serialize_character_string_size
+  (t: character_string_type)
+  // (lb: asn1_value_int32_of_type t)
+  // (ub: asn1_value_int32_of_type t { lb <= ub })
+  // (x: asn1_string_with_character_bound_t t (count_character t) lb ub)
+  (x: datatype_of_asn1_type t)
+: Lemma (
+    match t with
+    | IA5_STRING -> predicate_serialize_asn1_string_TLV_size
+                     (IA5_STRING)
+                     (dfst)
+                     (filter_asn1_ia5_string)
+                     (synth_asn1_ia5_string)
+                     (synth_asn1_ia5_string_inverse)
+                     (lemma_synth_asn1_ia5_string_injective ())
+                     (x)
+    | PRINTABLE_STRING
+                 -> predicate_serialize_asn1_string_TLV_size
+                     (PRINTABLE_STRING)
+                     (dfst)
+                     (filter_asn1_printable_string)
+                     (synth_asn1_printable_string)
+                     (synth_asn1_printable_string_inverse)
+                     (lemma_synth_asn1_printable_string_injective ())
+                     (x))
 = match t with
   | IA5_STRING ->
                   // assert_norm ( t == IA5_STRING /\
