src/riot/asn1/ASN1.Spec.Value.PRINTABLE_STRING.fsti
@@ -1,0 +1,160 @@
+module ASN1.Spec.Value.PRINTABLE_STRING
+
+open ASN1.Spec.Base
+
+open ASN1.Base
+open ASN1.Spec.Value.StringCombinator
+
+open FStar.Integers
+
+module B32 = FStar.Bytes
+
+(* ZT: Maybe we don't need to hide this module, which is
+       just instantiating another mudule. Since the lemmas'
+       types are also instantiating some meta predicates,
+       they are meanlingless unless a module friends this
+       module. *)
+
+let filter_asn1_printable_string
+  (len: asn1_value_int32_of_type PRINTABLE_STRING)
+  (s32: B32.lbytes32 len)
+: GTot (bool)
+= let s = B32.reveal s32 in
+  Seq.for_all valid_PRINTABLE_byte s
+
+val synth_asn1_printable_string
+  (len: asn1_value_int32_of_type PRINTABLE_STRING)
+  (s32: parse_filter_refine (filter_asn1_printable_string len))
+: GTot (value: datatype_of_asn1_type PRINTABLE_STRING{(dfst value) == len})
+
+val lemma_synth_asn1_printable_string_injective (_: unit)
+: Lemma (
+  forall (len: asn1_value_int32_of_type (PRINTABLE_STRING)).
+    synth_injective (synth_asn1_printable_string len)
+)
+
+noextract inline_for_extraction
+val synth_asn1_printable_string_inverse
+  (len: asn1_value_int32_of_type PRINTABLE_STRING)
+  (value: datatype_of_asn1_type PRINTABLE_STRING{(dfst value) == len})
+: (s32: parse_filter_refine (filter_asn1_printable_string len)
+             { value == synth_asn1_printable_string len s32 })
+
+(* ZT: Exposing those two since the type of lemmas below
+       depends on their implementation *)
+let parse_asn1_printable_string
+  (len: asn1_value_int32_of_type PRINTABLE_STRING)
+: parser (parse_asn1_string_kind PRINTABLE_STRING len)
+         (x: datatype_of_asn1_type PRINTABLE_STRING {dfst x == len})
+= parse_asn1_string
+    (PRINTABLE_STRING)
+    (dfst)
+    (filter_asn1_printable_string)
+    (synth_asn1_printable_string)
+    (lemma_synth_asn1_printable_string_injective ())
+    (len)
+
+let serialize_asn1_printable_string
+  (len: asn1_value_int32_of_type PRINTABLE_STRING)
+: serializer (parse_asn1_printable_string len)
+= serialize_asn1_string
+    (PRINTABLE_STRING)
+    (dfst)
+    (filter_asn1_printable_string)
+    (synth_asn1_printable_string)
+    (synth_asn1_printable_string_inverse)
+    (lemma_synth_asn1_printable_string_injective ())
+    (len)
+
+val lemma_serialize_asn1_printable_string_unfold
+  (len: asn1_value_int32_of_type PRINTABLE_STRING)
+  (x: datatype_of_asn1_type PRINTABLE_STRING { dfst x == len })
+: Lemma (
+  predicate_serialize_asn1_string_unfold
+    (PRINTABLE_STRING)
+    (dfst)
+    (filter_asn1_printable_string)
+    (synth_asn1_printable_string)
+    (synth_asn1_printable_string_inverse)
+    (lemma_synth_asn1_printable_string_injective ())
+    (len)
+    (x)
+)
+
+val lemma_serialize_asn1_printable_string_size
+  (len: asn1_value_int32_of_type PRINTABLE_STRING)
+  (x: datatype_of_asn1_type PRINTABLE_STRING { dfst x == len })
+: Lemma (
+  predicate_serialize_asn1_string_size
+    (PRINTABLE_STRING)
+    (dfst)
+    (filter_asn1_printable_string)
+    (synth_asn1_printable_string)
+    (synth_asn1_printable_string_inverse)
+    (lemma_synth_asn1_printable_string_injective ())
+    (len)
+    (x)
+)
+
+let parse_asn1_printable_string_TLV_kind = parse_asn1_string_TLV_kind PRINTABLE_STRING
+
+let parse_asn1_printable_string_TLV
+: parser parse_asn1_printable_string_TLV_kind (datatype_of_asn1_type PRINTABLE_STRING)
+= parse_asn1_string_TLV
+    (PRINTABLE_STRING)
+    (dfst)
+    (filter_asn1_printable_string)
+    (synth_asn1_printable_string)
+    (lemma_synth_asn1_printable_string_injective ())
+
+let serialize_asn1_printable_string_TLV
+: serializer (parse_asn1_printable_string_TLV)
+= serialize_asn1_string_TLV
+    (PRINTABLE_STRING)
+    (dfst)
+    (filter_asn1_printable_string)
+    (synth_asn1_printable_string)
+    (synth_asn1_printable_string_inverse)
+    (lemma_synth_asn1_printable_string_injective ())
+
+val lemma_serialize_asn1_printable_string_TLV_unfold
+  (x: datatype_of_asn1_type PRINTABLE_STRING)
+: Lemma (
+  predicate_serialize_asn1_string_TLV_unfold
+    (PRINTABLE_STRING)
+    (dfst)
+    (filter_asn1_printable_string)
+    (synth_asn1_printable_string)
+    (synth_asn1_printable_string_inverse)
+    (lemma_synth_asn1_printable_string_injective ())
+    (x)
+)
+
+val lemma_serialize_asn1_printable_string_TLV_size
+  (x: datatype_of_asn1_type PRINTABLE_STRING)
+: Lemma (
+  predicate_serialize_asn1_string_TLV_size
+    (PRINTABLE_STRING)
+    (dfst)
+    (filter_asn1_printable_string)
+    (synth_asn1_printable_string)
+    (synth_asn1_printable_string_inverse)
+    (lemma_synth_asn1_printable_string_injective ())
+    (x)
+)
+
+(* ZT: Consider to expose this if anything in `X509.BasicFields.RelativeDistinguishedName` got blocked. *)
+val count_printable_character
+  (x: datatype_of_asn1_type PRINTABLE_STRING)
+: (asn1_int32)
+
+val parse_asn1_printable_string_TLV_with_character_bound
+  (lb: asn1_value_int32_of_type PRINTABLE_STRING)
+  (ub: asn1_value_int32_of_type PRINTABLE_STRING { lb <= ub })
+: parser parse_asn1_printable_string_TLV_kind (asn1_string_with_character_bound_t PRINTABLE_STRING count_printable_character lb ub)
+
+val serialize_asn1_printable_string_TLV_with_character_bound
+  (lb: asn1_value_int32_of_type PRINTABLE_STRING)
+  (ub: asn1_value_int32_of_type PRINTABLE_STRING { lb <= ub })
+: serializer (parse_asn1_printable_string_TLV_with_character_bound lb ub)
+
